made the extractable ocaml code compiled. 1) defined sz, align, INT as different modules with enough operations, such that the module generativity can ensure that we wont misuse them with nat or Z.
2) fixed two issues of extraction (fixextract.py)
  a) if you have two modules in Coq, 
   Module Type A.
     Variable a: Set.
   End A.
   Module B <: A.
     Definition a := nat.
   End B.
   Module C <: A.
     Definition a := Z.
   End C.
  With realizing B.a and C.a to be different types
  The extracted Ocaml *.mli is
   Module A = Sig 
     type a 
   End A
   Module B : A.
   Module C : A.
  although *.ml assigns the different concrete types to B and C.
  b) used Obj.magic to force Ocaml to type check monad join that is too
polymorphic.

3) extracted Ocaml into separate modules, rather than a large file.



git-svn-id: https://webdav.seas.upenn.edu/svn/sol/vol@2685 eef5ea85-cc2e-0410-bd84-0fae1f012da8

src/Parser/main.ml
@@ -1,6 +1,6 @@
 open Printf
 open Llvm
-open Symexe
+open Symexe_correct
 
 let main in_filename out_filename =
 	let ic = create_context () in
@@ -33,3 +33,4 @@ let main in_filename out_filename =
 let () = match Sys.argv with
 	| [| _; in_filename; out_filename |] -> main in_filename out_filename
 	| _ -> main "Input.bc" "Output.bc"
+
