src/Parser/myocamlbuild.ml
@@ -7,7 +7,7 @@ ocaml_lib ~extern:true "llvm_target";;
 ocaml_lib ~extern:true "llvm_bitreader";;
 ocaml_lib ~extern:true "llvm_bitwriter";;
 ocaml_lib ~extern:true "llvm_scalar_opts";;
-ocaml_lib ~extern:true "symexe";;
+ocaml_lib ~extern:true "symexe_correct";;
 
 flag ["link"; "ocaml"; "g++"] (S[A"-cc"; A"g++"]);;
 dep ["link"; "ocaml"; "use_bindings"] ;;
