src/ssa/extraction/Llvmcaml.ml
@@ -1,0 +1,26 @@
+(* This function used at the proof to generate a fresh atom, which should not be used at runtime. *)
+let atom_fresh_for_list a = failwith "AtomImpl.atom_fresh_for_list cannot be used at runtime"
+
+(* These conversion functions are very efficient, because the machine representation of
+   nat is not practice. We should figure out if we can remove these functions later... *)
+let int2nat i = failwith "int2nat is undef"
+
+let nat2int i = failwith "nat2int is undef"
+
+let llapint2nat i = failwith "llapint2nat is undef"
+
+let llapint2z i = failwith "llapint2Z is undef"
+
+let nat2llapint i = failwith "nat2llapint is undef"
+
+(* The functions below use the above conversion functions, I hope we wont use them at runtime. *)
+let nth_list_typ i lt = failwith "nth_list_typ cannot be used at runtime"
+
+let getCmdTyp c = failwith "getCmdtyp cannot be used at runtime"
+
+let getTyp c = failwith "getTyp cannot be used at runtime"
+
+let getPrimitiveSizeInBits t = failwith "getPrimitiveSizeInBits cannot be used at runtime"
+
+let getNumElements t = failwith "getNumElements cannot be used at runtime"
+
