src/ssa/ssa_extract.v
@@ -1,5 +1,6 @@
 Add LoadPath "./ott".
 Add LoadPath "./monads".
+Add LoadPath "./compcert".
 (* Add LoadPath "../../../theory/metatheory". *)
 
 Require Import ssa_dynamic.
@@ -12,377 +13,103 @@ Require Import ssa_mem.
 Require Import Values.
 Require Import Memory.
 Require Import Integers.
+Require Import Floats.
 Require Import Coqlib.
+Require Import ssa.
+Require Import ssa_interpreter.
 
-Export LLVMopsem.
+Extract Inductive bool => "bool" [ "true" "false" ].
+Extract Inductive sumbool => "bool" [ "true" "false" ].
+Extract Inductive list => "list" [ "[]" "(::)" ].
+Extract Inductive prod => "(*)"  [ "(,)" ].
+Extract Inductive option => "option"  [ "Some" "None" ].
 
-Definition interInsn (state:State) : option (State*trace) :=
-(* Check if the stack is empty. *) 
-match state with
-| mkState Sys TD Ps nil gl Mem0 => None
-| mkState Sys TD Ps ((mkEC F B cs tmn lc arg0 als)::EC) gl Mem0 =>
-  (* If cs is nil, we check tmn, 
-     otherwise, we check the first cmd in cs *)
-  match cs with
-  | nil => (* terminator *)
-    match tmn with
-    | insn_return rid RetTy Result =>
-      (* the suspended stacks cannot be empty, and
-          there must be a caller of the current function. *)
-      match EC with
-      | nil => None
-      | (mkEC F' B' nil tmn' lc' arg' als')::EC'' => None
-      | (mkEC F' B' (c'::cs') tmn' lc' arg' als')::EC'' =>
-        (* there must be a caller of the current function. *)
-        if (Instruction.isCallInst c') 
-        then 
-          do Mem' <- free_allocas Mem0 als;
-             ret ((mkState Sys TD Ps ((mkEC F' B' cs' tmn' (returnUpdateLocals TD c' RetTy Result lc lc' gl) arg' als')::EC'') gl Mem'),
-                  trace_nil)
-        else None
-      end
-    | insn_return_void rid =>
-      (* the suspended stacks cannot be empty, and
-          there must be a caller of the current function. *)
-      match EC with
-      | nil => None
-      | (mkEC F' B' nil tmn' lc' arg' als')::EC'' => None
-      | (mkEC F' B' (c'::cs') tmn' lc' arg' als')::EC'' =>
-        (* there must be a caller of the current function. *)
-        if (Instruction.isCallInst c')
-        then
-          do Mem' <- free_allocas Mem0 als;
-             ret ((mkState Sys TD Ps ((mkEC F' B' cs' tmn' lc' arg' als')::EC'') gl Mem'),
-                  trace_nil)
-        else None
-      end
-    | insn_br bid Cond l1 l2 =>
-      (* read the value of Cond *)
-      do cond0 <- (getOperandInt TD 1 Cond lc gl);
-      (* look up the target block *)
-        match (if zeq (cond0:Z) 0
-               then lookupBlockViaLabelFromFdef F l2
-               else lookupBlockViaLabelFromFdef F l1) with
-        | None => None
-        | Some (block_intro l' ps' cs' tmn') =>
-            Some ((mkState Sys TD Ps ((mkEC F (block_intro l' ps' cs' tmn') cs' tmn' 
-                     (switchToNewBasicBlock (block_intro l' ps' cs' tmn') B lc) arg0 als)::EC) gl Mem0),
-                  trace_nil)
-        end
-    | insn_br_uncond bid l0 =>
-      (* look up the target block *)
-      match (lookupBlockViaLabelFromFdef F l0) with
-      | None => None
-      | Some (block_intro l' ps' cs' tmn') =>
-          Some ((mkState Sys TD Ps ((mkEC F (block_intro l' ps' cs' tmn') cs' tmn' 
-                        (switchToNewBasicBlock (block_intro l' ps' cs' tmn') B lc) arg0 als)::EC) gl Mem0),
-               trace_nil)
-      end
-    | insn_unreachable _ => None
-    end
+Extract Constant AtomImpl.atom => "String.t".
+Extract Constant AtomImpl.eq_atom_dec => "fun a b -> a == b".
+Extract Constant AtomImpl.atom_fresh_for_list => "Llvmcaml.atom_fresh_for_list".
 
-  | c::cs => (* non-terminator *)
-    match c with
-    | insn_bop id0 bop0 sz0 v1 v2 => 
-      do gv3 <- BOP TD lc gl bop0 sz0 v1 v2;
-         ret ((mkState Sys TD Ps ((mkEC F B cs tmn (updateAddAL _ lc id0 gv3) arg0 als)::EC) gl Mem0),
-              trace_nil)         
-    | insn_extractvalue id0 t v idxs =>
-      do gv <- getOperandValue TD v lc gl;
-      do gv' <- extractGenericValue TD t gv idxs;
-         ret ((mkState Sys TD Ps ((mkEC F B cs tmn (updateAddAL _ lc id0 gv') arg0 als)::EC) gl Mem0),
-              trace_nil)
-    | insn_insertvalue id0 t v t' v' idxs =>
-      do gv <- getOperandValue TD v lc gl;
-      do gv' <- getOperandValue TD v' lc gl;
-      do gv'' <- insertGenericValue TD t gv idxs t' gv';
-         ret ((mkState Sys TD Ps ((mkEC F B cs tmn (updateAddAL _ lc id0 gv'') arg0 als)::EC) gl Mem0),
-             trace_nil)
-    | insn_malloc id0 t sz0 align0 =>
-      do tsz <- getTypeAllocSize TD t;
-      match (malloc TD Mem0 (tsz * sz0)%nat align0) with
-      | None => None
-      | Some (Mem', mb) =>
-        ret ((mkState Sys TD Ps ((mkEC F B cs tmn (updateAddAL _ lc id0 (blk2GV TD mb)) arg0 als)::EC) gl Mem'),
-            trace_nil)
-      end
-    | insn_free fid t v =>
-      do mptr <- getOperandPtr TD v lc gl;
-      do Mem' <- free Mem0 mptr;
-         ret ((mkState Sys TD Ps ((mkEC F B cs tmn lc arg0 als)::EC) gl Mem'), trace_nil)
-    | insn_alloca id0 t sz0 align0 =>
-      do tsz <- getTypeAllocSize TD t;
-      match (malloc TD Mem0 (tsz * sz0)%nat align0) with
-      | None => None
-      | Some (Mem', mb) =>
-          ret ((mkState Sys TD Ps ((mkEC F B cs tmn (updateAddAL _ lc id0 (blk2GV TD mb)) arg0 (mb::als))::EC) gl Mem'),
-              trace_nil)
-      end
-    | insn_load id0 t v align0 =>
-      do mp <- getOperandPtr TD v lc gl;
-      do gv <- mload TD Mem0 mp t align0;
-         ret ((mkState Sys TD Ps ((mkEC F B cs tmn (updateAddAL _ lc id0 gv) arg0 als)::EC) gl Mem0),
-              trace_nil)
-    | insn_store sid t v1 v2 align0 =>
-      do gv1 <- getOperandValue TD v1 lc gl;
-      do mp2 <- getOperandPtr TD v2 lc gl;
-      do Mem' <- mstore TD Mem0 mp2 t gv1 align0;
-         ret ((mkState Sys TD Ps ((mkEC F B cs tmn lc arg0 als)::EC) gl Mem'),
-             trace_nil)
-    | insn_gep id0 inbounds0 t v idxs =>
-      do mp <- getOperandPtr TD v lc gl;
-      do mp' <- GEP TD lc gl t mp idxs inbounds0;
-         ret ((mkState Sys TD Ps ((mkEC F B cs tmn (updateAddAL _ lc id0 (ptr2GV TD mp')) arg0 als)::EC) gl Mem0),
-             trace_nil)
-    | insn_ext id0 extop0 t1 v1 t2 =>
-      do gv2 <- EXT TD lc gl extop0 t1 v1 t2;
-         ret ((mkState Sys TD Ps ((mkEC F B cs tmn (updateAddAL _ lc id0 gv2) arg0 als)::EC) gl Mem0),
-             trace_nil)
-    | insn_cast id0 castop0 t1 v1 t2 =>
-      do gv2 <- CAST TD lc gl castop0 t1 v1 t2;
-         ret ((mkState Sys TD Ps ((mkEC F B cs tmn (updateAddAL _ lc id0 gv2) arg0 als)::EC) gl Mem0),
-             trace_nil)
-    | insn_icmp id0 cond0 t v1 v2 =>
-      do gv3 <- ICMP TD lc gl cond0 t v1 v2;
-         ret ((mkState Sys TD Ps ((mkEC F B cs tmn (updateAddAL _ lc id0 gv3) arg0 als)::EC) gl Mem0),
-             trace_nil)
-    | insn_select id0 v0 t v1 v2 =>
-      do cond0 <- getOperandInt TD 1 v0 lc gl;
-      do gv1 <- getOperandValue TD v1 lc gl;
-      do gv2 <- getOperandValue TD v2 lc gl;
-         ret ((mkState Sys TD Ps ((mkEC F B cs tmn (if zeq (cond0:Z) 0 then updateAddAL _ lc id0 gv2 else updateAddAL _ lc id0 gv1) arg0 als)::EC) gl Mem0),
-             trace_nil)  
-    | insn_call rid noret0 tailc0 rt fid lp =>
-      (* only look up the current module for the time being, 
-         do not support linkage. *)
-      match (lookupFdefViaIDFromProducts Ps fid) with
-      | None => None
-      | Some (fdef_intro (fheader_intro rt' fid' la) lb) =>
-        if id_dec fid fid' then
-          if typ_dec rt rt' then
-            match (getEntryBlock (fdef_intro (fheader_intro rt fid la) lb)) with
-            | None => None
-            | Some (block_intro l' ps' cs' tmn') =>
-                ret ((mkState Sys TD Ps ((mkEC (fdef_intro (fheader_intro rt fid la) lb) 
-                                          (block_intro l' ps' cs' tmn') cs' tmn' (initLocals la (params2GVs TD lp lc gl)) 
-                                          (params2GVs TD lp lc gl) nil)::
-                                        (mkEC F B ((insn_call rid noret0 tailc0 rt fid lp)::cs) tmn lc arg0 als)::EC) gl Mem0),
-                    trace_nil)
-            end
-          else None
-        else None
-      end
-    end
-  end
-end.
+Extract Constant LLVMsyntax.id => "String.t".
+Extract Constant LLVMsyntax.l => "String.t".
+Extract Constant LLVMsyntax.inbounds => "bool".
+Extract Constant LLVMsyntax.tailc => "bool".
+Extract Constant LLVMsyntax.noret => "bool".
 
-Lemma dsInsn__implies__interInsn : forall state state' tr,
-  dsInsn state state' tr ->
-  interInsn state = Some (state', tr).
-Proof. 
-  intros state state' tr HdsInsn.
-  Opaque malloc. 
-  (dsInsn_cases (destruct HdsInsn) Case); simpl;
-    try solve [rewrite H; simpl; rewrite H0; simpl; rewrite H1; simpl; auto |
-               rewrite H; simpl; rewrite H0; simpl; auto |
-               rewrite H; simpl; auto ].
-  Case "dsBranch".
-    simpl. rewrite H. simpl. rewrite <- H0. simpl. auto.
-  Case "dsBranch_uncond".
-    simpl. rewrite <- H. simpl. auto.
-  Case "dsCall".
-    rewrite H. simpl in H0. rewrite H0. 
-    destruct (id_dec fid fid); auto.
-      destruct (typ_dec rt rt); auto.
-        contradict n; auto.
-      contradict n; auto.
-Qed.
+Extract Constant LLVMsyntax.Size.t => "int32".
+Extract Constant LLVMsyntax.Size.Zero => "0l".
+Extract Constant LLVMsyntax.Size.One => "1l".
+Extract Constant LLVMsyntax.Size.Two => "2l".
+Extract Constant LLVMsyntax.Size.Four => "4l".
+Extract Constant LLVMsyntax.Size.Eight => "8l".
+Extract Constant LLVMsyntax.Size.Sixteen => "16l".
+Extract Constant LLVMsyntax.Size.ThirtyTwo => "32l".
+Extract Constant LLVMsyntax.Size.SixtyFour => "64l".
+Extract Constant LLVMsyntax.Size.from_nat => "fun x -> Int32.of_int (Camlcoq.camlint_of_nat x)".
+Extract Constant LLVMsyntax.Size.to_nat => "Camlcoq.nat_of_camlint".
+Extract Constant LLVMsyntax.Size.to_Z => "Camlcoq.z_of_camlint".
+Extract Constant LLVMsyntax.Size.from_Z => "Camlcoq.camlint_of_z".
+Extract Constant LLVMsyntax.Size.add => "Int32.add".
+Extract Constant LLVMsyntax.Size.sub => "Int32.sub".
+Extract Constant LLVMsyntax.Size.mul => "Int32.mul".
+Extract Constant LLVMsyntax.Size.div => "Int32.div".
+Extract Constant LLVMsyntax.Size.dec => "fun (x:int32) (y:int32) -> Int32.compare x y == 0".
 
-Lemma interInsn__implies__dsInsn : forall state state' tr,
-  interInsn state = Some (state', tr) ->
-  dsInsn state state' tr.
-Proof.
-  intros state state' tr HinterInsn.
-  destruct state.
-  destruct ECS0; simpl in HinterInsn;
-    try solve [inversion HinterInsn].
+Extract Constant LLVMsyntax.Align.t => "int32".
+Extract Constant LLVMsyntax.Align.Zero => "0l".
+Extract Constant LLVMsyntax.Align.One => "1l".
+Extract Constant LLVMsyntax.Align.Two => "2l".
+Extract Constant LLVMsyntax.Align.Four => "4l".
+Extract Constant LLVMsyntax.Align.Eight => "8l".
+Extract Constant LLVMsyntax.Align.Sixteen => "16l".
+Extract Constant LLVMsyntax.Align.ThirtyTwo => "32l".
+Extract Constant LLVMsyntax.Align.SixtyFour => "64l".
+Extract Constant LLVMsyntax.Align.from_nat => "fun x -> Int32.of_int (Camlcoq.camlint_of_nat x)".
+Extract Constant LLVMsyntax.Align.to_nat => "Camlcoq.nat_of_camlint".
+Extract Constant LLVMsyntax.Align.to_Z => "Camlcoq.z_of_camlint".
+Extract Constant LLVMsyntax.Align.from_Z => "Camlcoq.camlint_of_z".
+Extract Constant LLVMsyntax.Align.add => "Int32.add".
+Extract Constant LLVMsyntax.Align.sub => "Int32.sub".
+Extract Constant LLVMsyntax.Align.mul => "Int32.mul".
+Extract Constant LLVMsyntax.Align.div => "Int32.div".
+Extract Constant LLVMsyntax.Align.dec => "fun (x:int32) (y:int32) -> Int32.compare x y == 0".
 
-    destruct e as [F B cs tmn lc arg0 als].
-    destruct cs.
-      destruct tmn.
-      Case "insn_return".
-        destruct ECS0;
-          try solve [inversion HinterInsn].
-          
-          destruct e as [F' B' cs' tmn' lc' arg' als'].
-          destruct cs';
-            try solve [inversion HinterInsn].
+Extract Constant LLVMsyntax.INTEGER.t => "Llvm.llapint".
+Extract Constant LLVMsyntax.INTEGER.to_nat => "Llvmcaml.llapint2nat".
+Extract Constant LLVMsyntax.INTEGER.to_Z => "Llvmcaml.llapint2z".
+Extract Constant LLVMsyntax.INTEGER.dec => "Llvm.APInt.compare".
 
-            remember (Instruction.isCallInst c) as R1.
-            remember (free_allocas Mem0 als) as R2.
-            destruct R1; try solve [inversion HinterInsn].
-            destruct R2; inversion HinterInsn; subst; eauto.
+Extract Constant LLVMlib.inbounds_dec => "(==)".
+Extract Constant LLVMlib.tailc_dec => "(==)".
+Extract Constant LLVMlib.noret_dec => "(==)".
 
-      Case "insn_return_void".
-        destruct ECS0;
-          try solve [inversion HinterInsn].
-          
-          destruct e as [F' B' cs' tmn' lc' arg' als'].
-          destruct cs';
-            try solve [inversion HinterInsn].
+(* Float *)
+Extract Inlined Constant Floats.float => "float".
+Extract Constant Floats.Float.zero   => "0.".
+(* Extract Constant Floats.Float.one   => "1.". *)
+Extract Constant Floats.Float.neg => "( ~-. )".
+Extract Constant Floats.Float.abs => "abs_float".
+Extract Constant Floats.Float.singleoffloat => "Floataux.singleoffloat".
+Extract Constant Floats.Float.intoffloat => "Floataux.intoffloat".
+Extract Constant Floats.Float.intuoffloat => "Floataux.intuoffloat".
+Extract Constant Floats.Float.floatofint => "Floataux.floatofint".
+Extract Constant Floats.Float.floatofintu => "Floataux.floatofintu".
+Extract Constant Floats.Float.add => "( +. )".
+Extract Constant Floats.Float.sub => "( -. )".
+Extract Constant Floats.Float.mul => "( *. )".
+Extract Constant Floats.Float.div => "( /. )".
+Extract Constant Floats.Float.cmp => "Floataux.cmp".
+Extract Constant Floats.Float.eq_dec => "fun (x: float) (y: float) -> x = y".
 
-            remember (Instruction.isCallInst c) as R1.
-            remember (free_allocas Mem0 als) as R2.
-            destruct R1; try solve [inversion HinterInsn].
-            destruct R2; inversion HinterInsn; subst; eauto.
+(* Memdata *)
+Extract Constant Memdata.big_endian => "Memdataaux.big_endian".
+Extract Constant Memdata.encode_float => "Memdataaux.encode_float".
+Extract Constant Memdata.decode_float => "Memdataaux.decode_float".
 
-      Case "insn_br".
-        remember (getOperandInt CurTargetData0 1 v lc Globals0) as R1.
-        destruct R1; try solve [inversion HinterInsn].
-          simpl in HinterInsn.
-          destruct (zeq z 0).
-            remember (lookupBlockViaLabelFromFdef F l1) as R2.
-            destruct R2; inversion HinterInsn; subst.
-              destruct b.
-              inversion HinterInsn; subst; eauto.
-        
-            remember (lookupBlockViaLabelFromFdef F l0) as R2.
-            destruct R2; inversion HinterInsn; subst.
-              destruct b.
-              inversion HinterInsn; subst.
-              eapply dsBranch; eauto.    
-                destruct (zeq z 0); auto.
-                  contradict e; auto.                
+(* Memory - work around an extraction bug. *)
+Extraction NoInline Memory.Mem.valid_pointer.
 
-      Case "insn_br_uncond".
-        remember (lookupBlockViaLabelFromFdef F l0) as R2.
-        destruct R2; inversion HinterInsn; subst.
-          destruct b.
-          inversion HinterInsn; subst; eauto.
+Extraction Blacklist List String Int.
 
-      Case "insn_unreachable".
-        inversion HinterInsn.
-                    
-      destruct c.
-      Case "insn_bop".
-        remember (BOP CurTargetData0 lc Globals0 b s v v0) as R1.
-        destruct R1; 
-          simpl in HinterInsn;
-          inversion HinterInsn; subst; eauto.
-          
-      Case "insn_extractvalue".
-        remember (getOperandValue CurTargetData0 v lc Globals0) as R1.
-        destruct R1; simpl in HinterInsn; 
-          try solve [inversion HinterInsn].         
-        remember (extractGenericValue CurTargetData0 t g l0) as R2.
-        destruct R2; simpl in HinterInsn; 
-          inversion HinterInsn; subst; eauto.
-
-      Case "insn_insertvalue".
-        remember (getOperandValue CurTargetData0 v lc Globals0) as R1.
-        destruct R1; simpl in HinterInsn; 
-          try solve [inversion HinterInsn].         
-        remember (getOperandValue CurTargetData0 v0 lc Globals0) as R2.
-        destruct R2; simpl in HinterInsn; 
-          try solve [inversion HinterInsn].         
-        remember (insertGenericValue CurTargetData0 t g l0 t0 g0) as R3.
-        destruct R3; simpl in HinterInsn; 
-          inversion HinterInsn; subst; eauto.
-          
-      Case "insn_malloc".
-        remember (getTypeAllocSize CurTargetData0 t) as R1.
-        destruct R1; simpl in HinterInsn; 
-          try solve [inversion HinterInsn].         
-        remember (malloc CurTargetData0 Mem0 (n*s)%nat a) as R2.
-        destruct R2; simpl in HinterInsn; 
-          try solve [inversion HinterInsn].         
-        destruct p; 
-          inversion HinterInsn; subst; eauto.
-          
-      Case "insn_free".
-        remember (getOperandPtr CurTargetData0 v lc Globals0) as R1.
-        destruct R1; simpl in HinterInsn; 
-          try solve [inversion HinterInsn].         
-        remember (free Mem0 v0) as R2.
-        destruct R2; simpl in HinterInsn; 
-          inversion HinterInsn; subst; eauto.
-          
-      Case "insn_alloca".
-        remember (getTypeAllocSize CurTargetData0 t) as R1.
-        destruct R1; simpl in HinterInsn; 
-          try solve [inversion HinterInsn].         
-        remember (malloc CurTargetData0 Mem0 (n*s)%nat a) as R2.
-        destruct R2; simpl in HinterInsn; 
-          try solve [inversion HinterInsn].         
-        destruct p; 
-          inversion HinterInsn; subst; eauto.
-          
-      Case "insn_load".
-        remember (getOperandPtr CurTargetData0 v lc Globals0) as R1.
-        destruct R1; simpl in HinterInsn; 
-          try solve [inversion HinterInsn].         
-        remember (mload CurTargetData0 Mem0 v0 t a) as R2.
-        destruct R2; simpl in HinterInsn; 
-          inversion HinterInsn; subst; eauto.
-          
-      Case "insn_store".
-        remember (getOperandValue CurTargetData0 v lc Globals0) as R1.
-        destruct R1; simpl in HinterInsn; 
-          try solve [inversion HinterInsn].         
-        remember (getOperandPtr CurTargetData0 v0 lc Globals0) as R2.
-        destruct R2; simpl in HinterInsn; 
-          try solve [inversion HinterInsn].         
-        remember (mstore CurTargetData0 Mem0 v1 t g a) as R3.
-        destruct R3; simpl in HinterInsn; 
-          inversion HinterInsn; subst; eauto.
-          
-      Case "insn_gep".
-        remember (getOperandPtr CurTargetData0 v lc Globals0) as R1.
-        destruct R1; simpl in HinterInsn; 
-          try solve [inversion HinterInsn].         
-        remember (GEP CurTargetData0 lc Globals0 t v0 l0 i1) as R2.
-        destruct R2; simpl in HinterInsn; 
-          inversion HinterInsn; subst; eauto.
-
-      Case "insn_ext".
-        remember (EXT CurTargetData0 lc Globals0 e t v t0) as R.
-        destruct R; simpl in HinterInsn; 
-          inversion HinterInsn; subst; eauto.
-
-      Case "insn_cast".
-        remember (CAST CurTargetData0 lc Globals0 c t v t0) as R.
-        destruct R; simpl in HinterInsn; 
-          inversion HinterInsn; subst; eauto.
-
-      Case "insn_icmp".
-        remember (ICMP CurTargetData0 lc Globals0 c t v v0) as R.
-        destruct R; simpl in HinterInsn; 
-          inversion HinterInsn; subst; eauto.
-
-      Case "insn_select".
-        remember (getOperandInt CurTargetData0 1 v lc Globals0) as R1.
-        destruct R1; simpl in HinterInsn; 
-          try solve [inversion HinterInsn].         
-        remember (getOperandValue CurTargetData0 v0 lc Globals0) as R2.
-        destruct R2; simpl in HinterInsn; 
-          try solve [inversion HinterInsn].         
-        remember (getOperandValue CurTargetData0 v1 lc Globals0) as R3.
-        destruct R3; simpl in HinterInsn; 
-          try solve [inversion HinterInsn].
-        inversion HinterInsn; subst; eauto.
-
-      Case "insn_call".
-        remember (lookupFdefViaIDFromProducts CurProducts0 i1) as R1.
-        destruct R1; simpl in HinterInsn; 
-          try solve [inversion HinterInsn].
-        destruct f. destruct f.
-        destruct (id_dec i1 i2); try solve [inversion HinterInsn]; subst.
-        destruct (typ_dec t0 t1); try solve [inversion HinterInsn]; subst.
-        destruct b; try solve [inversion HinterInsn].
-        destruct b.
-        inversion HinterInsn; subst; eauto.
-Qed.
-
-Extraction interInsn.
-
+Cd "extraction".
+Recursive Extraction Library ssa_interpreter.
+Cd "../".
 
